<?xml version="1.0" encoding="UTF-8"?>

<!DOCTYPE rdf:RDF [
    <!ENTITY owl "http://www.w3.org/2002/07/owl#" >
    <!ENTITY dc "http://purl.org/dc/elements/1.1/" >
    <!ENTITY xsd "http://www.w3.org/2001/XMLSchema#" >
    <!ENTITY rdfs "http://www.w3.org/2000/01/rdf-schema#" >
    <!ENTITY rdf "http://www.w3.org/1999/02/22-rdf-syntax-ns#" >
   	<!ENTITY co "http://purl.org/co#" > 	
]>

<rdf:RDF xmlns="https://www.eclipse.org/ice#"
	xmlns:adms="http://www.w3.org/ns/adms#"
	xmlns:skos="http://www.w3.org/2004/02/skos/core#"
	xmlns:rdf="http://www.w3.org/1999/02/22-rdf-syntax-ns#"
	xmlns:owl="http://www.w3.org/2002/07/owl#"
	xmlns:xsd="http://www.w3.org/2001/XMLSchema#"
	xmlns:co="http://purl.org/co#"
	xmlns:dc="http://purl.org/dc/elements/1.1/"
	xmlns:rdfs="http://www.w3.org/2000/01/rdf-schema#">

	<!-- ICE Ontology -->

	<owl:Ontology>
		<owl:versionInfo rdf:datatype="&xsd;string">1.0</owl:versionInfo>
		<dc:date rdf:datatype="&xsd;string">January 19, 2019</dc:date>
		<dc:contributor rdf:datatype="&xsd;string">Jay Jay Billings</dc:contributor>
		<dc:format rdf:datatype="&xsd;string">application/rdf+xml</dc:format>
		<dc:language>en</dc:language>
		<dc:title xml:lang="en">The Eclipse Integrated Environment Data
			Ontology</dc:title>
		<dc:creator rdf:resource="https://www.eclipse.org/ice" />
		<owl:imports
			rdf:resource="http://www.w3.org/2004/02/skos/core" />
		<owl:imports rdf:resource="http://purl.org/co" />
		<!-- <owl:imports rdf:resource="http://www.w3.org/ns/adms"/> -->
	</owl:Ontology>

	<!-- Identifiable, base of data hierarchy -->

	<rdf:Description
		rdf:about="https://www.eclipse.org/ice#Identifiable">
		<rdf:type rdf:resource="http://www.w3.org/2002/07/owl#Class" />
		<rdfs:comment xml:lang="en">This class describes objects that
			are identifiable to ICE.</rdfs:comment>
		<rdfs:label xml:lang="en">Identifiable</rdfs:label>
		<rdfs:subClassOf
			rdf:resource="http://www.w3.org/2002/07/owl#Thing" />
	</rdf:Description>

	<rdf:Description
		rdf:about="https://www.eclipse.org/ice#context">
		<rdf:type
			rdf:resource="http://www.w3.org/2002/07/owl#ObjectProperty" />
		<rdfs:comment xml:lang="en">The context can be thought of as
			an additional clue that can be provided with the object to allow
			clients to interpret its contents in a slightly different way.</rdfs:comment>
		<rdfs:domain
			rdf:resource="https://www.eclipse.org/ice#Identifiable" />
		<rdfs:label xml:lang="en">context</rdfs:label>
		<rdfs:range
			rdf:resource="http://www.w3.org/2002/07/owl#AnnotationProperty" />
	</rdf:Description>

	<rdf:Description
		rdf:about="https://www.eclipse.org/ice#identifier">
		<rdf:type
			rdf:resource="http://www.w3.org/2002/07/owl#ObjectProperty" />
		<rdfs:comment xml:lang="en">A unique identifier for the
			object.</rdfs:comment>
		<rdfs:domain
			rdf:resource="https://www.eclipse.org/ice#Identifiable" />
		<rdfs:label xml:lang="en">id</rdfs:label>
		<rdfs:range
			rdf:resource="http://www.w3.org/2001/XMLSchema#long" />
		<!-- <rdfs:range rdf:resource="http://www.w3.org/ns/adms#identifier"/> -->
	</rdf:Description>

	<rdf:Description
		rdf:about="https://www.eclipse.org/ice#name">
		<rdf:type
			rdf:resource="http://www.w3.org/2002/07/owl#ObjectProperty" />
		<rdfs:comment xml:lang="en">The name that should be given to
			the Identifiable entity.</rdfs:comment>
		<rdfs:domain
			rdf:resource="https://www.eclipse.org/ice#Identifiable" />
		<rdfs:label xml:lang="en">name</rdfs:label>
		<rdfs:range
			rdf:resource="http://www.w3.org/2001/XMLSchema#string" />
	</rdf:Description>

	<rdf:Description
		rdf:about="https://www.eclipse.org/ice#desc">
		<rdf:type
			rdf:resource="http://www.w3.org/2002/07/owl#ObjectProperty" />
		<rdfs:comment xml:lang="en">The description that should be
			given to the Identifiable entity.</rdfs:comment>
		<rdfs:domain
			rdf:resource="https://www.eclipse.org/ice#Identifiable" />
		<rdfs:label xml:lang="en">description</rdfs:label>
		<rdfs:range
			rdf:resource="http://www.w3.org/2001/XMLSchema#string" />
	</rdf:Description>

	<!-- Component - base of data-holding components such as data component, 
		etc. in Form -->

	<rdf:Description
		rdf:about="https://www.eclipse.org/ice#Component">
		<rdf:type rdf:resource="http://www.w3.org/2002/07/owl#Class" />
		<rdfs:comment xml:lang="en">Components are special types of
			Identifiables that manage or share data, and which act as nodes in
			the Form (a tree).</rdfs:comment>
		<rdfs:label xml:lang="en">Component</rdfs:label>
		<rdfs:subClassOf
			rdf:resource="https://www.eclipse.org/ice#Identifiable" />
	</rdf:Description>

	<!-- Composite - Root and parent nodes in Form (tree). -->

	<rdf:Description
		rdf:about="https://www.eclipse.org/ice#Composite">
		<rdf:type rdf:resource="http://www.w3.org/2002/07/owl#Class" />
		<rdfs:comment xml:lang="en">Composites hold collections of
			Components to store data and are the root and parent nodes in the
			Form data tree.</rdfs:comment>
		<rdfs:label xml:lang="en">Composite</rdfs:label>
		<rdfs:subClassOf
			rdf:resource="https://www.eclipse.org/ice#Component" />
	</rdf:Description>

	<!-- The class that defines the list of components found on the composite. -->
	
	<owl:Class
		rdf:about="https://www.eclipse.org/ice#ComponentList">
		<rdf:type rdf:resource="http://www.w3.org/2002/07/owl#Class" />
		<rdfs:comment xml:lang="en">The list of components associated
			with the composite.</rdfs:comment>
		<rdfs:label xml:lang="en">ComponentList</rdfs:label>
		<rdfs:subClassOf rdf:resource="http://purl.org/co#Seq" />
		<!-- Note that a second subClassOf block is required by the parser. Properties 
			cannot go in the first subClassOf block, apparently. Failure to do so will 
			cause Apache Jena, for example, to produce an error saying that "The attributes 
			on this property element, are not permitted with any content; expecting end 
			element tag." -->
		<rdfs:subClassOf>
			<!-- Restrict the element type of the list to be a Component -->
			<owl:Restriction>
				<owl:onProperty
					rdf:resource="http://purl.org/co/previousItem" />
				<rdfs:range
					rdf:resource="https://www.eclipse.org/ice#Component" />
			</owl:Restriction>
		</rdfs:subClassOf>
	</owl:Class>

	<!-- The property declaring the membership of and range relationship between 
		Composite and ComponentList. -->
	<owl:ObjectProperty
		rdf:about="https://www.eclipse.org/ice#componentListProperty">
		<rdfs:comment xml:lang="en">The link between the Composite and
			ComponentList.</rdfs:comment>
		<rdfs:domain
			rdf:resource="https://www.eclipse.org/ice#Composite" />
		<rdfs:label xml:lang="en">componentListProperty</rdfs:label>
		<rdfs:range
			rdf:resource="https://www.eclipse.org/ice#ComponentList"></rdfs:range>
	</owl:ObjectProperty>

</rdf:RDF> 