@prefix owl: <http://www.w3.org/2002/07/owl#> .
@prefix rdfs: <http://www.w3.org/2000/01/rdf-schema#> .
@prefix xsd: <http://www.w3.org/2001/XMLSchema#> .
@prefix dc11: <http://purl.org/dc/elements/1.1/> .
@prefix co: <http://purl.org/co> .
@prefix sh: <http://www.w3.org/ns/shacl#> .
@prefix rdf: <http://www.w3.org/1999/02/22-rdf-syntax-ns#> .
@prefix ice-data: <https://www.eclipse.org/ice/data#> .
@prefix ice-wf: <https://www.eclipse.org/ice/workflows#> .

Workflow Description:
links to data
> as resources - file, stream, URL, etc. Use dctype:Dataset
task list

What forms can data sets take? 
>Input data: sources, databases, etc.
>Output data: scratch, provenance, results, etc.
>Diagnostic data: logs

What's in a task?
>It's action (specified as a resource)
>Task-specific Parameters (specified as a resource)
>Where it runs
>When it runs
>Input data
>Output data

# ----- Basic workflow description and associated classes.

<https://www.eclipse.org/ice/workflows#WorkflowDescription>
  a owl:Class ;
  rdfs:comment """This class provides a description of the data and tasks that make up a workflow."""@en ;
  rdfs:label "Workflow Description"@en ;
  rdfs:subClassOf ice-data:Identifiable .
  
<https://www.eclipse.org/ice/workflows#TaskList>
  a co:List ;
  rdfs:comment """This is a list of tasks that should be executed in the workflow."""@en ;
  rdfs:label "Task list"@en ;
  rdfs:domain <https://www.eclipse.org/ice/workflows#WorkflowDescription> .

# ----- Actions that can be executed as part of tasks

<https://www.eclipse.org/ice/workflows#Action>
  rdfs:comment """This is an action that can be executed in a task of the workflow."""@en ;
  rdfs:label "Action"@en .

<https://www.eclipse.org/ice/workflows#ActionTarget>
  rdfs:comment """This tag describes the target (program, function, web service, etc.) that the action should execute."""@en ;
  rdfs:label "Action Target"@en ;
  rdfs:domain <https://www.eclipse.org/ice/workflows#Action> ;

<https://www.eclipse.org/ice/workflows#ActionType>
  rdfs:comment """This is a tag that describes the type of the action. This is generally specific to underlying workflow engines."""@en ;
  rdfs:label "Action Type"@en ;
  rdfs:domain <https://www.eclipse.org/ice/workflows#Action> ;
  rdfs:range xsd:string .

# ----- Ontology info

[]
  a owl:Ontology ;
  owl:versionInfo "1.0"^^xsd:string ;
  dc11:date "March 31, 2019"^^xsd:string ;
  dc11:contributor "Jay Jay Billings"^^xsd:string ;
  dc11:format "application/rdf+xml"^^xsd:string ;
  dc11:language "en" ;
  dc11:title """The Eclipse Integrated Environment Workflow
			Ontology"""@en ;
  dc11:creator <https://www.eclipse.org/ice> ;
  owl:imports <http://www.w3.org/2004/02/skos/core>, <http://purl.org/co> .
