@prefix owl: <http://www.w3.org/2002/07/owl#> .
@prefix rdfs: <http://www.w3.org/2000/01/rdf-schema#> .
@prefix xsd: <http://www.w3.org/2001/XMLSchema#> .
@prefix dc11: <http://purl.org/dc/elements/1.1/> .
@prefix co: <http://purl.org/co> .
@prefix sh: <http://www.w3.org/ns/shacl#> .
@prefix rdf: <http://www.w3.org/1999/02/22-rdf-syntax-ns#> .
@prefix ice: <https://www.eclipse.org/ice#> .

<https://www.eclipse.org/ice#Identifiable>
  a owl:Class ;
  rdfs:comment """This class describes objects that
			are identifiable to ICE."""@en ;
  rdfs:label "Identifiable"@en ;
  rdfs:subClassOf owl:Thing .

<https://www.eclipse.org/ice#context>
  a owl:ObjectProperty ;
  rdfs:comment """The context can be thought of as
			an additional clue that can be provided with the object to allow
			clients to interpret its contents in a slightly different way."""@en ;
  rdfs:domain <https://www.eclipse.org/ice#Identifiable> ;
  rdfs:label "context"@en ;
  rdfs:range owl:AnnotationProperty .

<https://www.eclipse.org/ice#identifier>
  a owl:ObjectProperty ;
  rdfs:comment """A unique identifier for the
			object."""@en ;
  rdfs:domain <https://www.eclipse.org/ice#Identifiable> ;
  rdfs:label "id"@en ;
  rdfs:range xsd:long .

<https://www.eclipse.org/ice#name>
  a owl:ObjectProperty ;
  rdfs:comment """The name that should be given to
			the Identifiable entity."""@en ;
  rdfs:domain <https://www.eclipse.org/ice#Identifiable> ;
  rdfs:label "name"@en ;
  rdfs:range xsd:string .

<https://www.eclipse.org/ice#desc>
  a owl:ObjectProperty ;
  rdfs:comment """The description that should be
			given to the Identifiable entity."""@en ;
  rdfs:domain <https://www.eclipse.org/ice#Identifiable> ;
  rdfs:label "description"@en ;
  rdfs:range xsd:string .

<https://www.eclipse.org/ice#Component>
  a owl:Class ;
  rdfs:comment """Components are special types of
			Identifiables that manage or share data, and which act as nodes in
			the Form (a tree)."""@en ;
  rdfs:label "Component"@en ;
  rdfs:subClassOf <https://www.eclipse.org/ice#Identifiable> .

<https://www.eclipse.org/ice#Composite>
  a owl:Class ;
  rdfs:comment """Composites hold collections of
			Components to store data and are the root and parent nodes in the
			Form data tree."""@en ;
  rdfs:label "Composite"@en ;
  rdfs:subClassOf <https://www.eclipse.org/ice#Component> .

<https://www.eclipse.org/ice#ComponentList>
  a owl:Class ;
  rdfs:comment """The list of components associated
			with the composite."""@en ;
  rdfs:label "ComponentList"@en ;
  rdfs:subClassOf <http://purl.org/co#Set>.
  
<https://www.eclipse.org/ice#ComponentListShape>
  a sh:NodeShape ;
  sh:targetClass <https://www.eclipse.org/ice#ComponentList> ; 
  sh:property [
	sh:path co:element ;
	sh:class <https://www.eclipse.org/ice#Component> ;
	sh:nodeKind sh:IRI ;
  ] ;
  sh:closed true ;
  sh:ignoredProperties (rdf:type) .

<https://www.eclipse.org/ice#componentListProperty>
  a owl:ObjectProperty ;
  rdfs:comment """The link between the Composite and
			ComponentList."""@en ;
  rdfs:domain <https://www.eclipse.org/ice#Composite> ;
  rdfs:label "componentListProperty"@en ;
  rdfs:range <https://www.eclipse.org/ice#ComponentList> .

[]
  a owl:Ontology ;
  owl:versionInfo "1.0"^^xsd:string ;
  dc11:date "January 19, 2019"^^xsd:string ;
  dc11:contributor "Jay Jay Billings"^^xsd:string ;
  dc11:format "application/rdf+xml"^^xsd:string ;
  dc11:language "en" ;
  dc11:title """The Eclipse Integrated Environment Data
			Ontology"""@en ;
  dc11:creator <https://www.eclipse.org/ice> ;
  owl:imports <http://www.w3.org/2004/02/skos/core>, <http://purl.org/co> .
